% Chapter 2: Foundations of Frourio Analysis
\chapter{Foundations of Frourio Analysis}
\label{chap:frourio_analysis}

\section{The Golden Ratio}
\label{sec:golden_ratio}

\begin{definition}[Golden Ratio]
\label{def:golden_ratio}
\lean{FUST.phi, FUST.psi}
\leanok
\[
\varphi = \frac{1+\sqrt{5}}{2}, \quad \psi = \frac{1-\sqrt{5}}{2}
\]
\end{definition}

\section{Frourio Exponential Function}
\label{sec:frourio_exp}

\begin{definition}[Fibonacci Factorial]
\label{def:fib_factorial}
Define the Fibonacci factorial as $n!_{\mathsf{F}} := \prod_{k=1}^{n} F_k$.
\end{definition}

\begin{definition}[Frourio Exponential]
\label{def:frourio_exp}
\[
\exp_{\mathsf{F}}(x) = \sum_{n=0}^{\infty} \frac{x^n}{n!_{\mathsf{F}}}
\]
\end{definition}

\section{Frourio Constant}
\label{sec:frourio_constant}

\begin{definition}[Frourio Constant]
\label{def:frourio_constant}
\[
\mathfrak{f} := \exp_{\mathsf{F}}(1) = \sum_{n=0}^{\infty} \frac{1}{n!_{\mathsf{F}}} \approx 3.7045
\]
\end{definition}

\textbf{Alternative representation} (Binet type):
\[
\mathfrak{f} = \frac{\exp_{\mathsf{F}}(\varphi) - \exp_{\mathsf{F}}(\psi)}{\sqrt{5}} = \frac{D_2[\exp_{\mathsf{F}}](1)}{\sqrt{5}}
\]

This is a constant that gives a natural scale to the golden ratio.

\section{Fibonacci Decomposition}
\label{sec:fib_decomposition}

\begin{theorem}[Fibonacci Decomposition]
\label{thm:fib_decomposition}
\lean{FUST.phi_pow_fib}
\leanok
For any integer $k$,
\[
\varphi^k = F_k\varphi + F_{k-1}, \quad \psi^k = F_k\psi + F_{k-1}
\]
where $F_k$ is the Fibonacci sequence.
\end{theorem}

\begin{proof}
By induction.
\begin{itemize}
\item $k=0$: $\varphi^0 = 1 = 0 \cdot \varphi + 1$.
\item $k=1$: $\varphi^1 = 1 \cdot \varphi + 0$.
\item $k \to k+1$: $\varphi^{k+1} = \varphi(F_k\varphi + F_{k-1}) = F_k(\varphi+1) + F_{k-1}\varphi = F_{k+1}\varphi + F_k$.
\end{itemize}
\end{proof}

\section{Binet Formula}
\label{sec:binet}

\begin{theorem}[Binet Formula]
\label{thm:binet}
\lean{FUST.binet_formula}
\leanok
For any integer $k$,
\[
\varphi^k - \psi^k = F_k \cdot \sqrt{5}
\]
\end{theorem}

\begin{proof}
From $\varphi^k = F_k\varphi + F_{k-1}$ and $\psi^k = F_k\psi + F_{k-1}$, we have
$\varphi^k - \psi^k = F_k(\varphi - \psi) = F_k \sqrt{5}$.
\end{proof}
